Specify and prove an initial blockchain semantics
This specifies an initial version of blockchain semantics. The semantics
are specified as several relations:

ChainStep :
  Environment -> Action -> Tx ->
  Environment -> list Action ->
  Prop.

This relation captures the semantics of a single step/action in the
chain. Such an action can either be a transfer, contract deployment or
contract call. It specifies that when an action is executed in some
starting environment, then the blockchain records a transaction (Tx) on
the chain and performs certain updates to the environment. Finally, the
step also results in possible new actions to be executed due to contract
execution.

An environment is for now simply a Chain (which contracts can interact
with) and a collection of contracts that have been deployed to some
addresses. The Chain contains various useful operations for contracts
such as the current block number or ability to query transactions and
user balances.

For example, for a simple transfer action we may have ChainStep pre act
tx post []. Then the ChainStep relation will capture that the only thing
that has changed in the post environment is that tx has been added to
the chain (so that the appropriate account balances have been updated),
but for instance also that no new contracts have appeared. Since this is
just a transfer, there also cannot be any new actions to execute.

The semantics of the environment updates are captured in an abstract
manner to allow for different implementations of blockchains.
Specifically, we use an equivalence relation
EnvironmentEquiv : Environment -> Environment -> Prop and just require
that the environment is equivalent (under this relation) to an obvious
implementation of an environment. We implement an obvious blockchain,
LocalBlockchain, which uses finite maps with log n access times rather
than the linear maps used in the default semantics.

A single block, when added to a blockchain, consists of a list of these
actions to execute. In each block this list of actions must then be
executed (in a correct manner) until no more actions are left. This is
captured in
BlockTrace :
  Environment -> list Action ->
  Environment -> list Action -> Prop.
For all intents and purposes this can be seen as just a transitive
reflexive closure of the ChainStep relation above. Right now it only
allows blocks to reduce steps in a depth-first order, but this relation
should be simple to update to other or more general orders of reduction.
Note that ChainStep and BlockTrace say nothing about new blocks, but
only about execution within blocks. The semantics of how blocks are
added to the chain is captured in
ChainTrace : Environment -> Environment -> Prop.

This is a collection of block traces and representing additions of
blocks. At each block added, ChainTrace also captures that the
environment must be updated accordingly so that contracts can access
information about block numbers correctly.

Finally, a blockchain must always be able to prove that there is a
ChainTrace from its initial environment (the genesis blockchain) to its
current environment.

There are several TODOs left in the semantics:
1. We need to account for gas and allow execution failures
2. We need to put restrictions on when contracts can appear as the
source of actions
3. We need to capture soundness of the add_block function in blockchain
implementations

We also provide to sanity checks for these semantics:
1. We prove them for a simple block chain (LocalBlockchain.v).
2. We prove a "circulation" theorem for any blockchain satisfying the
semantics. That is, we show the following theorem:

Theorem chain_trace_circulation
      {env_start env_end : Environment}
      (trace : ChainTrace env_start env_end)
  : circulation env_end =
    (circulation env_start +
     coins_created
       (block_height (block_header env_start))
       (block_height (block_header env_end)))%Z.

src/Blockchain.v
@@ -1,29 +1,60 @@
+From Coq Require Import Arith ZArith.
 From Coq Require Import List.
+From Coq Require Import Psatz.
+From Coq Require Import Permutation.
+From Coq Require Import Morphisms.
+From Coq Require Import Setoid.
 From SmartContracts Require Import Oak.
 From SmartContracts Require Import Monads.
 From SmartContracts Require Import Extras.
+From SmartContracts Require Import Automation.
+From RecordUpdate Require Import RecordUpdate.
+From stdpp Require countable.
 
-Definition Address := nat.
+Import ListNotations.
+
+Definition Version := nat.
+
+Definition Amount := Z.
+
+Bind Scope Z_scope with Amount.
+
+Class ChainBaseTypes :=
+  build_chain_base_types {
+    Address : Type;
+    address_eqb : Address -> Address -> bool;
+    address_eqb_spec : forall (a b : Address), Bool.reflect (a = b) (address_eqb a b);
+    address_eqdec :> stdpp.base.EqDecision Address;
+    address_countable :> countable.Countable Address;
+    address_ote :> OakTypeEquivalence Address;
+    compute_block_reward : nat -> Amount;
+  }.
+
+Global Opaque Address address_eqb address_eqb_spec
+       address_eqdec address_countable
+       address_ote
+       compute_block_reward.
+
 Delimit Scope address_scope with address.
 Bind Scope address_scope with Address.
+Infix "=?" := address_eqb (at level 70) : address_scope.
 
-Module Address.
-  Definition eqb := Nat.eqb.
-End Address.
+Global Ltac destruct_address_eq :=
+  repeat
+    match goal with
+    | [|- context[(?a =? ?b)%address]] => destruct (address_eqb_spec a b)
+    end.
 
-Infix "=?" := Address.eqb (at level 70) : address_scope.
-
-Definition Amount := nat.
-Definition BlockId := nat.
-Definition Version := nat.
+Section Blockchain.
+Context {BaseTypes : ChainBaseTypes}.
 
 Record ContractDeployment :=
   build_contract_deployment {
     deployment_version : Version;
     (* todo: model any type/constraints so we can have this. Right now the
-       problem is that Congress messages can contain _any_ oak value (for
-       the congress to send out), so there is no bijection from its message type
-       to oak type.
+problem is that Congress messages can contain _any_ oak value (for
+the congress to send out), so there is no bijection from its message type
+to oak type.
     deployment_msg_ty : OakType;
     deployment_state_ty : OakType; *)
     deployment_setup : OakValue;
@@ -44,79 +75,80 @@ Record Tx :=
 
 Record BlockHeader :=
   build_block_header {
-    block_number : BlockId;
+    block_height : nat;
+    slot_number : nat;
+    finalized_height : nat;
   }.
 
-Record Block :=
-  build_block {
-    block_header : BlockHeader;
-    block_txs : list Tx;
-  }.
-
-(* The ChainInterface is an interface that allows different implementations
-of chains. This represents the view of the blockchain that a contract
-can access and interact with. This does not contain all information of
-the chain (and it can't for positivity reasons).
-*)
-Record ChainInterface :=
-  build_chain_interface {
-    (* Would be nice to encapsulate ChainInterface somewhat here
-       and avoid these ugly prefixed names *)
-    ci_type : Type;
-    ci_chain_at : ci_type -> BlockId -> option ci_type;
-    (* Last finished block. During contract execution, this is the previous
-       block, i.e. this block does _not_ contain the transaction that caused
-       the contract to be called *)
-    ci_head_block : ci_type -> Block;
-    ci_incoming_txs : ci_type -> Address -> list Tx;
-    ci_outgoing_txs :  ci_type -> Address -> list Tx;
-    ci_contract_state : ci_type -> Address -> option OakValue;
-  }.
-
-(* An actual chain interface together with a value of the chain.
-For example, one obvious chain implementation could be as a list
-of blocks and some operations on such a list. Then, the value is
-simply the list of blocks.
-This avoids having to either
-1. Import an actual instance of ChainInterface when taking a chain, or
-2. Abstracting over any implementation of ChainInterface when taking
-a chain. *)
+(* This represents the view of the blockchain that a contract
+can access and interact with. *)
 Record Chain :=
   build_chain {
-    chain_ci : ChainInterface;
-    chain_val : chain_ci.(ci_type);
+    block_header : BlockHeader;
+    incoming_txs : Address -> list Tx;
+    outgoing_txs : Address -> list Tx;
+    blocks_baked : Address -> list nat;
+    contract_state : Address -> option OakValue;
   }.
 
-Section ChainAccessors.
-  Context (chain : Chain).
+Record ChainEquiv (c1 c2 : Chain) : Prop :=
+  build_chain_equiv {
+    header_eq : block_header c1 = block_header c2;
+    incoming_txs_eq : forall addr, incoming_txs c1 addr = incoming_txs c2 addr;
+    outgoing_txs_eq : forall addr, outgoing_txs c1 addr = outgoing_txs c2 addr;
+    blocks_baked_eq : forall addr, blocks_baked c1 addr = blocks_baked c2 addr;
+    contract_state_eq : forall addr, contract_state c1 addr = contract_state c2 addr;
+  }.
 
-  Let g {A : Type} (p : forall chain : ChainInterface, ci_type chain -> A)
-      := p chain.(chain_ci) chain.(chain_val).
+Global Program Instance chain_equiv_equivalence : Equivalence ChainEquiv.
+Next Obligation.
+  intros x; apply build_chain_equiv; reflexivity.
+Qed.
+Next Obligation.
+  intros x y eq.
+  destruct eq; apply build_chain_equiv; congruence.
+Qed.
+Next Obligation.
+  intros x y z eq_xy eq_yz.
+  destruct eq_xy, eq_yz; apply build_chain_equiv; congruence.
+Qed.
 
-  Definition chain_at (bid : BlockId) : option Chain :=
-    do x <- chain.(chain_ci).(ci_chain_at) chain.(chain_val) bid;
-      Some {| chain_val := x |}.
+Global Instance chain_equiv_header_proper :
+  Proper (ChainEquiv ==> eq) block_header.
+Proof. intros x y. apply header_eq. Qed.
+Global Instance chain_equiv_incoming_txs_proper :
+  Proper (ChainEquiv ==> eq ==> eq) incoming_txs.
+Proof. intros x y eq a b eq'; subst; apply incoming_txs_eq; assumption. Qed.
+Global Instance chain_equiv_outgoing_txs_proper :
+  Proper (ChainEquiv ==> eq ==> eq) outgoing_txs.
+Proof. intros x y eq a b eq'; subst; apply outgoing_txs_eq; assumption. Qed.
+Global Instance chain_equiv_blocks_backes_proper :
+  Proper (ChainEquiv ==> eq ==> eq) blocks_baked.
+Proof. intros x y eq a b eq'; subst; apply blocks_baked_eq; assumption. Qed.
+Global Instance chain_equiv_contract_state_proper :
+  Proper (ChainEquiv ==> eq ==> eq) contract_state.
+Proof. intros x y eq a b eq'; subst; apply contract_state_eq; assumption. Qed.
 
-  Definition head_block := g ci_head_block.
-  Definition incoming_txs := g ci_incoming_txs.
-  Definition outgoing_txs := g ci_outgoing_txs.
-  Definition contract_state := g ci_contract_state.
-  Definition account_balance (addr : Address) : Amount :=
-    let sum := fold_right Nat.add 0 in
-    let sum_amounts txs := sum (map tx_amount txs) in
-    sum_amounts (incoming_txs addr) - sum_amounts (outgoing_txs addr).
-  Definition contract_deployment (addr : Address) : option ContractDeployment :=
-    let to_dep tx := match tx.(tx_body) with
-                     | tx_deploy dep => Some dep
-                     | _ => None
-                     end in
-    find_first to_dep (incoming_txs addr).
-End ChainAccessors.
+Section Accessors.
+Local Open Scope Z.
 
-Inductive ContractCallContext :=
-  build_contract_call_ctx {
-    (* Chain *)
-    ctx_chain : Chain;
+Definition account_balance (chain : Chain) (addr : Address)
+  : Amount :=
+  let sum_amounts txs := sumZ tx_amount txs in
+  sum_amounts (incoming_txs chain addr) - sum_amounts (outgoing_txs chain addr) +
+  sumZ compute_block_reward (blocks_baked chain addr).
+
+Definition contract_deployment (chain : Chain) (addr : Address)
+  : option ContractDeployment :=
+  let to_dep tx := match tx.(tx_body) with
+                  | tx_deploy dep => Some dep
+                  | _ => None
+                  end in
+  find_first to_dep (incoming_txs chain addr).
+End Accessors.
+
+Record ContractCallContext :=
+  build_ctx {
     (* Address sending the funds *)
     ctx_from : Address;
     (* Address of the contract being called *)
@@ -125,12 +157,13 @@ Inductive ContractCallContext :=
     ctx_amount : Amount;
   }.
 
-(* Operations that a contract can return that allows it to perform
-different actions as a result of its execution. *)
-Inductive ChainAction :=
+(* Operations that a contract can return or that a user can use
+to interact with a chain. *)
+Inductive ActionBody :=
   | act_transfer (to : Address) (amount : Amount)
   | act_call (to : Address) (amount : Amount) (msg : OakValue)
   | act_deploy (amount : Amount) (c : WeakContract) (setup : OakValue)
+
 (* Since one operation is the possibility to deploy a new contract,
 this represents an instance of a contract. Note that the act of deploying
 a contract has to be a separate thing to the contract deployment a contract
@@ -145,75 +178,143 @@ where Address -> WeakContract would be some operation that the chain provides
 to allow access to contracts in deployments.
 *)
 with WeakContract :=
-     | build_weak_contract
-         (version : Version)
-         (init : ContractCallContext -> OakValue -> option OakValue)
-         (receive : ContractCallContext -> OakValue (* state *) ->
-                    option OakValue (* message *) ->
-                    option (OakValue * list ChainAction)).
+    | build_weak_contract
+        (version : Version)
+        (init : Chain ->
+             ContractCallContext ->
+             OakValue ->
+             option OakValue)
+        (init_proper :
+           Proper (ChainEquiv ==> eq ==> eq ==> eq) init)
+        (receive :
+           Chain ->
+             ContractCallContext ->
+             OakValue (* state *) ->
+             option OakValue (* message *) ->
+             option (OakValue * list ActionBody))
+        (receive_proper :
+           Proper (ChainEquiv ==> eq ==> eq ==> eq ==> eq) receive).
+
+Definition wc_version (wc : WeakContract) : Version :=
+  let (v, _, _, _, _) := wc in v.
+
+Definition wc_init (wc : WeakContract) :=
+  let (_, i, _, _, _) := wc in i.
+
+Definition wc_init_proper (wc : WeakContract) :=
+  match wc return
+        Proper (ChainEquiv ==> eq ==> eq ==> eq) (wc_init wc) with
+  | build_weak_contract _ _ ip _ _ => ip
+  end.
+
+Definition wc_receive (wc : WeakContract) :=
+  let (_, _, _, r, _) := wc in r.
+
+Definition wc_receive_proper (wc : WeakContract) :=
+  match wc return
+        Proper (ChainEquiv ==> eq ==> eq ==> eq ==> eq) (wc_receive wc) with
+  | build_weak_contract _ _ _ _ rp => rp
+  end.
+
+Record Action :=
+  build_act {
+    act_from : Address;
+    act_body : ActionBody;
+  }.
 
 (* Represents a strongly-typed contract. This is what user's will primarily
 use and interact with when they want deployment. We keep the weak contract
 only "internally" for blockchains, while any strongly-typed contract can
 be converted to and from *)
 Record Contract
-       (setup_ty msg_ty state_ty : Type)
-       `{OakTypeEquivalence setup_ty}
-       `{OakTypeEquivalence msg_ty}
-       `{OakTypeEquivalence state_ty} :=
+      (setup_ty msg_ty state_ty : Type)
+      `{setup_eq : OakTypeEquivalence setup_ty}
+      `{msg_eq : OakTypeEquivalence msg_ty}
+      `{state_eq : OakTypeEquivalence state_ty} :=
   build_contract {
     version : Version;
-    init : ContractCallContext -> setup_ty -> option state_ty;
+    init :
+      Chain ->
+      ContractCallContext ->
+      setup_ty ->
+      option state_ty;
+    init_proper :
+      Proper (ChainEquiv ==> eq ==> eq ==> eq) init;
     receive :
-      ContractCallContext -> state_ty ->
-      option msg_ty -> option (state_ty * list ChainAction);
+      Chain ->
+      ContractCallContext ->
+      state_ty ->
+      option msg_ty ->
+      option (state_ty * list ActionBody);
+    receive_proper :
+      Proper (ChainEquiv ==> eq ==> eq ==> eq ==> eq) receive;
   }.
 
-Arguments version {_ _ _ _ _ _} contract : rename.
-Arguments init {_ _ _ _ _ _} contract ctx setup : rename.
-Arguments receive {_ _ _ _ _ _} contract ctx state msg : rename.
+Arguments version {_ _ _ _ _ _}.
+Arguments init {_ _ _ _ _ _}.
+Arguments receive {_ _ _ _ _ _}.
 Arguments build_contract {_ _ _ _ _ _}.
 
-Definition contract_to_weak_contract
-           {setup_ty msg_ty state_ty : Type}
-           `{OakTypeEquivalence setup_ty}
-           `{OakTypeEquivalence msg_ty}
-           `{OakTypeEquivalence state_ty}
-           (c : Contract setup_ty msg_ty state_ty) : WeakContract :=
-  let weak_init ctx oak_setup :=
-      do setup <- deserialize oak_setup;
-      do state <- c.(init) ctx setup;
-      Some (serialize state) in
-  let weak_recv ctx oak_state oak_msg_opt :=
-      do state <- deserialize oak_state;
-      match oak_msg_opt with
-      | Some oak_msg =>
-        do msg <- deserialize oak_msg;
-        do '(new_state, acts) <- c.(receive) ctx state (Some msg);
-        Some (serialize new_state, acts)
-      | None =>
-        do '(new_state, acts) <- c.(receive)  ctx state None;
-        Some (serialize new_state, acts)
-      end in
-  build_weak_contract c.(version) weak_init weak_recv.
+Program Definition contract_to_weak_contract
+          {setup_ty msg_ty state_ty : Type}
+          `{setup_eq : OakTypeEquivalence setup_ty}
+          `{msg_eq : OakTypeEquivalence msg_ty}
+          `{state_eq : OakTypeEquivalence state_ty}
+          (c : Contract setup_ty msg_ty state_ty) : WeakContract :=
+      let weak_init chain ctx oak_setup :=
+          do setup <- deserialize oak_setup;
+          do state <- c.(init) chain ctx setup;
+          Some (serialize state) in
+      let weak_recv chain ctx oak_state oak_msg_opt :=
+          do state <- deserialize oak_state;
+          match oak_msg_opt with
+          | Some oak_msg =>
+            do msg <- deserialize oak_msg;
+            do '(new_state, acts) <- c.(receive) chain ctx state (Some msg);
+            Some (serialize new_state, acts)
+          | None =>
+            do '(new_state, acts) <- c.(receive) chain ctx state None;
+            Some (serialize new_state, acts)
+          end in
+      build_weak_contract c.(version) weak_init _ weak_recv _.
+Next Obligation.
+  intros.
+  intros c1 c2 eq_chains ctx1 ctx2 eq_ctx setup1 setup2 eq_setups.
+  subst ctx2 setup2.
+  subst weak_init.
+  simpl.
+  destruct (deserialize setup1); auto; simpl.
+  now rewrite init_proper.
+Qed.
+Next Obligation.
+  intros.
+  intros c1 c2 eq_chains ctx1 ctx2 eq_ctx state1 state2 eq_states msg1 msg2 eq_msgs.
+  subst ctx2 state2 msg2.
+  subst weak_recv.
+  simpl.
+  destruct (deserialize state1); auto; simpl.
+  destruct msg1.
+  + destruct (deserialize o); auto; simpl.
+    now rewrite receive_proper.
+  + now rewrite receive_proper.
+Qed.
 
 Coercion contract_to_weak_contract : Contract >-> WeakContract.
 
 (* Deploy a strongly typed contract with some amount and setup *)
 Definition create_deployment
-           {setup_ty msg_ty state_ty : Type}
-           `{OakTypeEquivalence setup_ty}
-           `{OakTypeEquivalence msg_ty}
-           `{OakTypeEquivalence state_ty}
-           (amount : Amount)
-           (contract : Contract setup_ty msg_ty state_ty)
-           (setup : setup_ty)
-  : ChainAction :=
+          {setup_ty msg_ty state_ty : Type}
+          `{OakTypeEquivalence setup_ty}
+          `{OakTypeEquivalence msg_ty}
+          `{OakTypeEquivalence state_ty}
+          (amount : Amount)
+          (contract : Contract setup_ty msg_ty state_ty)
+          (setup : setup_ty) : ActionBody :=
   act_deploy amount contract (serialize setup).
 
 (* The contract interface is the main mechanism allowing a deployed
 contract to interact with another deployed contract. This hides
-the ugly details everything being OakValue away from contracts. *)
+the ugly details of everything being OakValue away from contracts. *)
 Record ContractInterface {setup_ty msg_ty state_ty : Type} :=
   build_contract_interface {
     (* The address of the contract being interfaced with *)
@@ -225,22 +326,21 @@ Record ContractInterface {setup_ty msg_ty state_ty : Type} :=
     (* Obtain the state at some point of time *)
     get_state : Chain -> option state_ty;
     (* Make an action transferring money to the contract without
-       a message *)
-    transfer : Amount -> ChainAction;
+      a message *)
+    transfer : Amount -> ActionBody;
     (* Make an action calling the contract *)
-    call : Amount -> msg_ty -> ChainAction;
+    call : Amount -> msg_ty -> ActionBody;
   }.
 
 Arguments ContractInterface _ _ _ : clear implicits.
-Arguments build_contract_interface {_ _ _}.
 
 Definition get_contract_interface
-           (chain : Chain)
-           (addr : Address)
-           (setup_ty msg_ty state_ty : Type)
-           `{OakTypeEquivalence setup_ty}
-           `{OakTypeEquivalence msg_ty}
-           `{OakTypeEquivalence state_ty}
+          (chain : Chain)
+          (addr : Address)
+          (setup_ty msg_ty state_ty : Type)
+          `{OakTypeEquivalence setup_ty}
+          `{OakTypeEquivalence msg_ty}
+          `{OakTypeEquivalence state_ty}
   : option (ContractInterface setup_ty msg_ty state_ty) :=
   do 'build_contract_deployment ver ov_setup <- contract_deployment chain addr;
   do setup <- deserialize ov_setup;
@@ -254,88 +354,354 @@ Definition get_contract_interface
           transfer := ifc_transfer;
           call := ifc_call; |}.
 
-(* TODO: Is there a more organic way of doing this than duplicating the
-structures? Maybe by abstracting over the details or something? This is
-super ugly.*)
-Inductive FullTxBody :=
-  | ftx_empty
-  | ftx_deploy (contract : WeakContract) (setup : OakValue)
-  | ftx_call (message : OakValue).
+End Blockchain.
 
-Record FullTx :=
-  build_ftx {
-    ftx_from : Address;
-    ftx_to : Address;
-    ftx_amount : Amount;
-    ftx_body : FullTxBody;
-    ftx_is_internal : bool;
+Section Semantics.
+Context {BaseTypes : ChainBaseTypes}.
+
+Instance chain_settable : Settable _ :=
+  settable! build_chain
+  < block_header;
+    incoming_txs;
+    outgoing_txs;
+    blocks_baked;
+    contract_state >.
+
+Definition add_tx_to_map (addr : Address) (tx : Tx) (map : Address -> list Tx)
+  : Address -> list Tx :=
+  fun a => if address_eqb a addr
+           then tx :: map a
+           else map a.
+
+Definition set_chain_contract_state
+           (addr : Address) (state : OakValue) (map : Address -> option OakValue)
+  : Address -> option OakValue :=
+  fun a => if address_eqb a addr
+           then Some state
+           else map a.
+
+Record Environment :=
+  build_env {
+    env_chain :> Chain;
+    env_contracts : Address -> option WeakContract;
   }.
 
-Definition full_tx_to_tx (ftx : FullTx) : Tx :=
-  let (from, to, amount, fbody, _) := ftx in
-  let body :=
-      match fbody with
-      | ftx_empty => tx_empty
-      | ftx_deploy (build_weak_contract ver _ _) setup =>
-        tx_deploy (build_contract_deployment ver setup)
-      | ftx_call msg => tx_call msg
-      end in
-  build_tx from to amount body.
-
-Coercion full_tx_to_tx : FullTx >-> Tx.
-
-(* A ChainBuilder represents the additional state, operations and specifications
-that a concrete implementation of a block chain needs to support. In contrast
-to Chain and ChainInterface, this contains the _full_ blockchain information.
-Thus, a ChainBuilder should be convertible into a Chain but not vice-versa.
-As an example, the builder needs to contain information about all contracts
-(including their receive functions) to be able to properly call into contracts
-when receiving messages. The ChainBuilder is what supports the actual
-"progression of time" induced by new blocks being added. Such a ChainBuilder is
-what contracts will reason over when proving interesting temporal properties
-of their behavior. *)
-(* TODO: Naming of this is kind of bad. It is somewhat descriptive, but not really.
-   Maybe something like ChainEnvironment or ChainContext could be better. *)
-Record ChainBuilderInterface :=
-  build_chain_builder_interface {
-    cbi_chain_interface :> ChainInterface;
-    cbi_type : Type;
-    cbi_chain : cbi_type -> cbi_chain_interface.(ci_type);
-    cbi_initial : cbi_type;
-    cbi_add_block : cbi_type -> (* cur *)
-                    Address (* coinbase *) ->
-                    list (Address * ChainAction) (* actions *) ->
-                    option cbi_type;
-    (* List of transactions that have been executed on the chain, in order.
-That is, the head of the list corresponds to actions in the very first block.
-This includes "internal" transactions (txs resulting from contract execution) *)
-    cbi_all_txs : cbi_type -> list FullTx;
+Record EnvironmentEquiv (e1 e2 : Environment) : Prop :=
+  build_env_equiv {
+    chain_equiv :> ChainEquiv e1 e2;
+    contracts_eq : forall a, env_contracts e1 a = env_contracts e2 a;
   }.
 
-Record ChainBuilder :=
-  build_chain_builder {
-    chain_builder_cbi : ChainBuilderInterface;
-    chain_builder_val : chain_builder_cbi.(cbi_type);
+Global Program Instance environment_equiv_equivalence : Equivalence EnvironmentEquiv.
+Next Obligation.
+  intros x; apply build_env_equiv; reflexivity.
+Qed.
+Next Obligation.
+  intros x y []; apply build_env_equiv; now symmetry.
+Qed.
+Next Obligation.
+  intros x y z [] []; apply build_env_equiv; try congruence.
+  apply (@transitivity Chain _ _ _ y _); auto.
+Qed.
+
+Instance environment_equiv_contracts_proper (addr : Address) :
+  Proper (EnvironmentEquiv ==> eq ==> eq) env_contracts.
+Proof. repeat intro; subst; apply contracts_eq; assumption. Qed.
+
+Instance env_settable : Settable _ :=
+  settable! build_env <env_chain; env_contracts>.
+
+Definition update_chain (upd : Chain -> Chain) (e : Environment)
+  : Environment :=
+  let chain := env_chain e in
+  let chain := upd chain in
+  e <|env_chain := chain|>.
+
+Definition add_tx (tx : Tx) :=
+  update_chain (fun c =>
+                  c <|incoming_txs ::= add_tx_to_map (tx_to tx) tx|>
+                    <|outgoing_txs ::= add_tx_to_map (tx_from tx) tx|>).
+
+Definition add_contract (addr : Address) (contract : WeakContract) (e : Environment)
+  : Environment :=
+  e <| env_contracts ::=
+    fun f a =>
+      if address_eqb a addr
+      then Some contract
+      else f a |>.
+
+Definition set_contract_state (addr : Address) (state : OakValue) :=
+  update_chain
+    (fun c => c <|contract_state ::= set_chain_contract_state addr state|>).
+
+Section Step.
+Local Open Scope Z.
+(* Next we define a single step. It specifies how an external action
+changes an environment and which external actions to execute after it. *)
+(* todo: handle deploy/call failures. We should still transfer gas and allow this
+to be recorded. *)
+Inductive ChainStep :
+  Environment -> Action -> Tx ->
+  Environment -> list Action -> Prop :=
+  | step_empty :
+      forall {pre : Environment}
+             {act : Action}
+             {tx : Tx}
+             {new_env : Environment}
+             (from to : Address)
+             (amount : Amount),
+        amount <= account_balance pre from ->
+        env_contracts pre to = None ->
+        act = build_act from (act_transfer to amount) ->
+        tx = build_tx from to amount tx_empty ->
+        EnvironmentEquiv new_env (add_tx tx pre) ->
+        ChainStep pre act tx new_env []
+  | step_deploy :
+      forall {pre : Environment}
+             {act : Action}
+             {tx : Tx}
+             {new_env : Environment}
+             (from to : Address)
+             (amount : Amount)
+             (wc : WeakContract)
+             (setup : OakValue)
+             (state : OakValue),
+      amount <= account_balance pre from ->
+      env_contracts pre to = None ->
+      incoming_txs pre to = [] ->
+      act = build_act from (act_deploy amount wc setup) ->
+      tx = build_tx from to amount (tx_deploy (build_contract_deployment (wc_version wc) setup)) ->
+      wc.(wc_init)
+           (add_tx tx pre)
+           (build_ctx from to amount)
+           setup = Some state ->
+      EnvironmentEquiv
+        new_env
+        (set_contract_state to state (add_contract to wc (add_tx tx pre))) ->
+      ChainStep pre act tx new_env []
+  | step_call_empty :
+      forall {pre : Environment}
+             {act : Action}
+             {tx : Tx}
+             {new_env : Environment}
+             {new_acts : list Action}
+             (from to : Address)
+             (amount : Amount)
+             (wc : WeakContract)
+             (prev_state : OakValue)
+             (new_state : OakValue)
+             (resp_acts : list ActionBody),
+      amount <= account_balance pre from ->
+      env_contracts pre to = Some wc ->
+      contract_state pre to = Some prev_state ->
+      act = build_act from (act_transfer to amount) ->
+      tx = build_tx from to amount tx_empty ->
+      wc.(wc_receive)
+           (add_tx tx pre)
+           (build_ctx from to amount)
+           prev_state
+           None = Some (new_state, resp_acts) ->
+      new_acts = map (build_act to) resp_acts ->
+      EnvironmentEquiv
+        new_env
+        (set_contract_state to new_state (add_tx tx pre)) ->
+      ChainStep pre act tx new_env new_acts
+  | step_call_msg :
+      forall {pre : Environment}
+             {act : Action}
+             {tx : Tx}
+             {new_env : Environment}
+             {new_acts : list Action}
+             (from to : Address)
+             (amount : Amount)
+             (wc : WeakContract)
+             (msg : OakValue)
+             (prev_state : OakValue)
+             (new_state : OakValue)
+             (resp_acts : list ActionBody),
+      amount <= account_balance pre from ->
+      env_contracts pre to = Some wc ->
+      contract_state pre to = Some prev_state ->
+      act = build_act from (act_call to amount msg) ->
+      tx = build_tx from to amount (tx_call msg) ->
+      wc.(wc_receive)
+           (add_tx tx pre)
+           (build_ctx from to amount)
+           prev_state
+           (Some msg) = Some (new_state, resp_acts) ->
+      new_acts = map (build_act to) resp_acts ->
+      EnvironmentEquiv
+        new_env
+        (set_contract_state to new_state (add_tx tx pre)) ->
+      ChainStep pre act tx new_env new_acts.
+
+Context {pre : Environment} {act : Action} {tx : Tx}
+        {post : Environment} {new_acts : list Action}
+        (step : ChainStep pre act tx post new_acts).
+
+Lemma account_balance_post (addr : Address) :
+  (account_balance post addr =
+  account_balance pre addr
+  + (if (addr =? tx_to tx)%address then tx_amount tx else 0)
+  - (if (addr =? tx_from tx)%address then tx_amount tx else 0)).
+Proof.
+  unfold account_balance.
+  destruct step;
+    match goal with
+    | [H: EnvironmentEquiv _ _ |- _] => rewrite (H : ChainEquiv _ _)
+    end;
+    simpl; unfold add_tx_to_map; destruct_address_eq; simpl; lia.
+Qed.
+
+Lemma account_balance_post_to :
+  tx_from tx <> tx_to tx ->
+  account_balance post (tx_to tx) =
+  account_balance pre (tx_to tx) + tx_amount tx.
+Proof.
+  rewrite account_balance_post.
+  destruct_address_eq; prove.
+Qed.
+
+Lemma account_balance_post_from :
+  tx_from tx <> tx_to tx ->
+  account_balance post (tx_from tx) =
+  account_balance pre (tx_from tx) - tx_amount tx.
+Proof.
+  rewrite account_balance_post.
+  destruct_address_eq; prove.
+Qed.
+
+Lemma account_balance_post_irrelevant (addr : Address) :
+  addr <> tx_from tx ->
+  addr <> tx_to tx ->
+  account_balance post addr = account_balance pre addr.
+Proof.
+  rewrite account_balance_post.
+  destruct_address_eq; prove.
+Qed.
+
+Lemma block_header_post_step : block_header post = block_header pre.
+Proof.
+  destruct step;
+    match goal with
+    | [H: EnvironmentEquiv _ _ |- _] => now rewrite (chain_equiv _ _ H)
+    end.
+Qed.
+End Step.
+
+(* A block trace is essentially just the reflexive transitive closure of the steps.
+It captures execution within a single block. *)
+Inductive BlockTrace :
+  Environment -> list Action ->
+  Environment -> list Action -> Prop :=
+  | btrace_refl : forall {acts} {env : Environment},
+      BlockTrace env acts env acts
+  | btrace_step : forall {pre post} act tx mid new_acts acts final,
+      ChainStep pre act tx mid new_acts ->
+      BlockTrace mid (new_acts ++ acts) post final ->
+      BlockTrace pre (act :: acts) post final.
+
+Section BlockTraceTheories.
+Context {pre : Environment} {acts : list Action}
+        {post : Environment} {post_acts : list Action}
+        (trace : BlockTrace pre acts post post_acts).
+
+Lemma block_header_post_steps : block_header post = block_header pre.
+Proof.
+  induction trace as [|? ? ? ? ? ? ? ? step prev_trace IH]; auto.
+  rewrite <- (block_header_post_step step).
+  auto.
+Qed.
+End BlockTraceTheories.
+
+Definition add_new_block
+          (header : BlockHeader)
+          (baker : Address)
+          (env : Environment) : Environment :=
+let chain := env_chain env in
+let chain :=
+    {| block_header := header;
+       incoming_txs := incoming_txs chain;
+       outgoing_txs := outgoing_txs chain;
+       contract_state := contract_state chain;
+       blocks_baked a :=
+         if address_eqb a baker
+         then block_height header :: blocks_baked chain a
+         else blocks_baked chain a; |} in
+env <|env_chain := chain|>.
+
+Definition IsValidNextBlock (new old : BlockHeader) : Prop :=
+  block_height new = S (block_height old) /\
+  slot_number new > slot_number old /\
+  finalized_height new >= finalized_height old /\
+  finalized_height new < block_height new.
+
+Inductive ChainTrace : Environment -> Environment -> Prop :=
+  | ctrace_refl : forall (env : Environment),
+      ChainTrace env env
+  | ctrace_block :
+      forall (prev_start prev_end : Environment)
+             (header : BlockHeader)
+             (baker : Address)
+             (acts : list Action)
+             (block_start new_end : Environment),
+        ChainTrace prev_start prev_end ->
+        IsValidNextBlock header (block_header prev_end) ->
+        BlockTrace block_start acts new_end [] ->
+        (* todo: probably unnecessary as we should have *)
+        (* BlockTrace a acts b acts' -> EnvironmentEquiv a a' -> *)
+        (* BlockTrace a' acts b acts' *)
+        EnvironmentEquiv
+          block_start
+          (add_new_block header baker prev_end) ->
+        ChainTrace prev_start new_end.
+
+Section ChainTraceTheories.
+Context {pre post : Environment} (trace : ChainTrace pre post).
+
+Lemma block_height_post_trace :
+  block_height (block_header pre) <= block_height (block_header post).
+Proof.
+  induction trace as [| ? ? ? ? ? ? ? ? ? valid block_trace eq]; auto.
+  apply le_trans with (block_height (block_header prev_end)); auto.
+  rewrite (block_header_post_steps block_trace).
+  rewrite (chain_equiv _ _ eq).
+  unfold IsValidNextBlock in valid.
+  simpl.
+  lia.
+Qed.
+End ChainTraceTheories.
+End Semantics.
+
+Section Blockchain.
+Context {BaseTypes : ChainBaseTypes}.
+
+Class ChainBuilderType :=
+  build_builder {
+    builder_type : Type;
+
+    builder_initial : builder_type;
+
+    builder_env : builder_type -> Environment;
+
+    builder_add_block
+      (b : builder_type)
+      (baker : Address)
+      (actions : list Action)
+      (slot_number : nat)
+      (finalized_height : nat) :
+      option builder_type;
+
+    builder_trace (b : builder_type) :
+      ChainTrace (builder_env builder_initial) (builder_env b);
   }.
 
-Definition chain_builder_chain (cb : ChainBuilder) : Chain :=
-  let (cbi, val) := cb in
-  build_chain cbi (cbi.(cbi_chain) val).
+Global Coercion builder_type : ChainBuilderType >-> Sortclass.
+End Blockchain.
 
-Coercion chain_builder_chain : ChainBuilder >-> Chain.
-
-Definition initial_chain_builder (cbi : ChainBuilderInterface) : ChainBuilder :=
-  build_chain_builder cbi cbi.(cbi_initial).
-
-Definition add_block
-           (cur : ChainBuilder)
-           (coinbase : Address)
-           (actions : list (Address * ChainAction))
-           : option ChainBuilder :=
-  let (ifc, val) := cur in
-  let new_val := ifc.(cbi_add_block) val coinbase actions in
-  option_map (build_chain_builder ifc) new_val.
-
-Definition all_txs (cb : ChainBuilder) :=
-  let (ifc, val) := cb in
-  ifc.(cbi_all_txs) val.
+Arguments version {_ _ _ _ _ _ _}.
+Arguments init {_ _ _ _ _ _ _}.
+Arguments receive {_ _ _ _ _ _ _}.
+Arguments build_contract {_ _ _ _ _ _ _}.
+Arguments ContractInterface {_} _ _ _.
+Arguments build_contract_interface {_ _ _ _}.
