src/Extras.v
@@ -1,4 +1,10 @@
+From Coq Require Import ZArith.
 From Coq Require Import List.
+From Coq Require Import Permutation.
+From Coq Require Import Morphisms.
+From Coq Require Import Psatz.
+From Coq Require Import Eqdep_dec.
+From SmartContracts Require Import Automation.
 Import ListNotations.
 
 Fixpoint find_first {A B : Type} (f : A -> option B) (l : list A)
@@ -20,3 +26,115 @@ Fixpoint map_option {A B : Type} (f : A -> option B) (l : list A)
                 end
   | [] => []
   end.
+
+Definition with_default {A : Type} (a : A) (o : option A) : A :=
+  match o with
+  | Some v => v
+  | None => a
+  end.
+
+
+Fixpoint sumZ {A : Type} (f : A -> Z) (xs : list A) : Z :=
+  match xs with
+  | [] => 0
+  | x :: xs' => f x + sumZ f xs'
+  end.
+
+Lemma sumZ_permutation
+      {A : Type} {f : A -> Z} {xs ys : list A}
+      (perm_eq : Permutation xs ys) :
+  sumZ f xs = sumZ f ys.
+Proof. induction perm_eq; prove. Qed.
+
+Instance sumZ_perm_proper {A : Type} {f : A -> Z} :
+  Proper (Permutation (A:=A) ==> eq) (sumZ f).
+Proof. intros x y perm. now apply sumZ_permutation. Qed.
+
+Local Open Scope Z.
+Lemma sumZ_app
+      {A : Type} {f : A -> Z} {xs ys : list A} :
+  sumZ f (xs ++ ys) = sumZ f xs + sumZ f ys.
+Proof.
+  revert ys.
+  induction xs as [| x xs IH]; intros ys; auto.
+  simpl.
+  rewrite IH.
+  lia.
+Qed.
+
+Lemma in_app_cons_or {A : Type} (x y : A) (xs ys : list A) :
+  x <> y ->
+  In x (xs ++ y :: ys) ->
+  In x (xs ++ ys).
+Proof.
+  intros x_neq_y x_in.
+  apply in_or_app.
+  apply in_app_or in x_in.
+  prove.
+Qed.
+
+Lemma incl_split {A : Type} (l m n : list A) :
+  incl (l ++ m) n -> incl l n /\ incl m n.
+Proof. unfold incl; generalize in_or_app; prove. Qed.
+
+Lemma NoDup_incl_reorganize
+      {A : Type}
+      (l l' : list A) :
+  NoDup l' ->
+  incl l' l ->
+  exists suf, Permutation (l' ++ suf) l.
+Proof.
+  revert l.
+  induction l' as [| x xs IH]; intros l nodup_l' incl_l'_l.
+  - exists l. apply Permutation_refl.
+  - assert (x_in_l: In x l).
+    + apply (incl_l'_l x). left. constructor.
+    + destruct (in_split _ _ x_in_l) as [pref [suf eq]]; subst.
+      inversion nodup_l'; subst.
+      assert (incl xs (pref ++ suf)).
+      * intros a a_in.
+        apply in_or_app.
+        apply (incl_split [x] xs _) in incl_l'_l.
+        destruct incl_l'_l as [incl_x incl_xs].
+        intuition.
+        specialize (incl_xs a a_in).
+        apply in_app_or in incl_xs.
+        destruct incl_xs as [in_pref | [in_x | in_suf]]; prove.
+      * destruct (IH _ H2 H) as [suf' perm_suf'].
+        exists suf'.
+        simplify_perm.
+Qed.
+
+Lemma in_NoDup_app {A : Type} (x : A) (l m : list A) :
+  In x l -> NoDup (l ++ m) -> ~In x m.
+Proof.
+  intros in_x_l nodup_l_app_m in_x_m.
+  destruct (in_split _ _ in_x_l) as [l1 [l2 eq]]; subst.
+  replace ((l1 ++ x :: l2) ++ m) with (l1 ++ x :: (l2 ++ m)) in nodup_l_app_m;
+    [|prove].
+  apply (NoDup_remove_2 _ _ _) in nodup_l_app_m.
+  rewrite app_assoc in nodup_l_app_m.
+  generalize in_or_app; prove.
+Qed.
+
+Lemma seq_app start len1 len2 :
+  seq start (len1 + len2) = seq start len1 ++ seq (start + len1) len2.
+Proof.
+  revert start.
+  induction len1 as [| len1 IH]; intros start.
+  - now rewrite Nat.add_0_r.
+  - simpl.
+    rewrite IH.
+    f_equal; f_equal; f_equal.
+    lia.
+Qed.
+
+Lemma sumZ_seq_S f start len :
+  sumZ f (seq start (S len)) = sumZ f (seq start len) + f (start + len)%nat.
+Proof.
+  replace (S len) with (len + 1)%nat by lia.
+  rewrite (seq_app start len 1).
+  rewrite sumZ_app.
+  simpl.
+  lia.
+Qed.
