src/BoundedN.v
@@ -1,0 +1,268 @@
+From Coq Require Import NArith ZArith.
+From SmartContracts Require Import Monads.
+From SmartContracts Require Import Finite.
+From SmartContracts Require Import Extras.
+From SmartContracts Require Import Automation.
+From Coq Require Import Eqdep_dec.
+From Coq Require Import List.
+From Coq Require Import Psatz.
+From Coq Require Import JMeq.
+From stdpp Require countable.
+Import ListNotations.
+
+Local Open Scope N.
+
+Inductive BoundedN (bound : N) :=
+  | bounded (n : N) (_ : (bound ?= n) = Gt).
+
+Arguments bounded {_}.
+
+Module BoundedN.
+  Definition to_N {bound : N} (n : BoundedN bound) : N :=
+    let (val, _) := n in val.
+
+  Definition eqb {bound : N} (a b : BoundedN bound) : bool :=
+    N.eqb (to_N a) (to_N b).
+
+  Definition of_N_compare {bound : N} (n : N) : option ((bound ?= n) = Gt) :=
+    match bound ?= n as comp return (option (comp = Gt)) with
+    | Gt => Some eq_refl
+    | _ => None
+    end.
+
+  Definition of_N {bound : N} (n : N) : option (BoundedN bound) :=
+    match of_N_compare n with
+    | Some prf => Some (bounded n prf)
+    | None => None
+    end.
+
+  Definition to_nat {bound : N} (n : BoundedN bound) : nat :=
+    N.to_nat (to_N n).
+
+  Definition of_nat {bound : N} (n : nat) : option (BoundedN bound) :=
+    of_N (N.of_nat n).
+
+  Definition to_Z {bound : N} (n : BoundedN bound) : Z :=
+    Z.of_N (to_N n).
+
+  Definition of_Z {bound : N} (z : Z) : option (BoundedN bound) :=
+    if (z <? 0)%Z then None else of_N (Z.to_N z).
+
+  Definition of_Z_const (bound : N) (z : Z) :=
+    let ofz := @of_Z bound z in
+    match ofz return (match ofz with
+                      | Some _ => BoundedN bound
+                      | None => unit
+                      end) with
+    | Some x => x
+    | None => tt
+    end.
+
+  Lemma to_N_inj {bound : N} {a b : BoundedN bound} :
+    to_N a = to_N b -> a = b.
+  Proof.
+    intros eq.
+    destruct a, b.
+    simpl in *.
+    subst.
+    f_equal.
+    apply UIP_dec.
+    decide equality.
+  Qed.
+
+  Hint Resolve to_N_inj.
+
+  Lemma eqb_spec {bound : N} (a b : BoundedN bound) :
+    Bool.reflect (a = b) (eqb a b).
+  Proof.
+    unfold eqb.
+    destruct (N.eqb_spec (to_N a) (to_N b)) as [eq | neq].
+    - constructor.
+      auto.
+    - constructor.
+      intros H; rewrite H in neq; tauto.
+  Qed.
+
+  Lemma eqb_refl {bound : N} (n : BoundedN bound) :
+    eqb n n = true.
+  Proof. destruct (eqb_spec n n); tauto. Qed.
+
+  Lemma to_nat_inj {bound : N} (a b : BoundedN bound) :
+    to_nat a = to_nat b -> a = b.
+  Proof.
+    intros eq.
+    apply to_N_inj.
+    unfold to_nat in eq.
+    now apply N2Nat.inj.
+  Qed.
+
+  Lemma to_Z_inj {bound : N} (a b : BoundedN bound) :
+    to_Z a = to_Z b -> a = b.
+  Proof.
+    intros eq.
+    apply to_N_inj.
+    unfold to_Z in eq.
+    now apply N2Z.inj.
+  Qed.
+
+  Lemma of_to_N {bound : N} (n : BoundedN bound) :
+    of_N (to_N n) = Some n.
+  Proof.
+    destruct n as [n prf]; simpl.
+    unfold of_N.
+    replace (of_N_compare n) with (Some prf); auto.
+    unfold of_N_compare.
+    now rewrite prf.
+  Qed.
+
+  Lemma of_to_nat {bound : N} (n : BoundedN bound) :
+    of_nat (to_nat n) = Some n.
+  Proof.
+    unfold to_nat, of_nat.
+    rewrite N2Nat.id.
+    apply of_to_N.
+  Qed.
+
+  Lemma of_n_not_lt_0 (n : N) :
+    (Z.of_N n <? 0)%Z = false.
+  Proof.
+    destruct (Z.ltb_spec (Z.of_N n) 0).
+    - apply Zlt_not_le in H.
+      destruct (H (N2Z.is_nonneg n)).
+    - reflexivity.
+  Qed.
+
+  Lemma of_to_Z {bound : N} (n : BoundedN bound) :
+    of_Z (to_Z n) = Some n.
+  Proof.
+    unfold to_Z, of_Z.
+    rewrite of_n_not_lt_0.
+    rewrite N2Z.id.
+    apply of_to_N.
+  Qed.
+
+  Lemma of_N_some {bound : N} {m : N} {n : BoundedN bound} :
+    of_N m = Some n -> to_N n = m.
+  Proof.
+    intros H.
+    unfold of_N in H.
+    destruct (of_N_compare m); try congruence.
+    now inversion H.
+  Qed.
+
+  Lemma of_N_none {bound : N} {m : N} :
+    @of_N bound m = None -> bound <= m.
+  Proof.
+    intros H.
+    unfold of_N in H.
+    destruct (of_N_compare m) eqn:comp; try congruence.
+    unfold of_N_compare in comp.
+    destruct (bound ?= m) eqn:comp'; congruence.
+  Qed.
+
+  Lemma of_nat_some {bound : N} {m : nat} {n : BoundedN bound} :
+    of_nat m = Some n -> to_nat n = m.
+  Proof.
+    intros H.
+    unfold to_nat.
+    rewrite (of_N_some H).
+    apply Nat2N.id.
+  Qed.
+
+  Lemma of_nat_none {bound : N} {m : nat} :
+    @of_nat bound m = None -> bound <= N.of_nat m.
+  Proof. apply of_N_none. Qed.
+
+  Lemma in_map_of_nat (bound : N) (n : BoundedN bound) (xs : list nat) :
+    In n (map_option (@of_nat bound) xs) <-> In (to_nat n) xs.
+  Proof.
+    induction xs as [|x xs IH].
+    - split; intros H; inversion H.
+    - simpl.
+      destruct (of_nat x) eqn:of_nat_x; split; intros H.
+      + destruct H.
+        * subst.
+          left.
+          symmetry.
+          now apply of_nat_some.
+        * tauto.
+      + destruct H as [eq | Hin].
+        * left.
+          rewrite eq in of_nat_x.
+          rewrite of_to_nat in of_nat_x; prove.
+        * prove.
+      + tauto.
+      + destruct H as [eq | Hin].
+        * rewrite eq, of_to_nat in of_nat_x; inversion of_nat_x.
+        * prove.
+  Qed.
+
+  Module Stdpp.
+    Import countable.
+    Lemma eq_dec {bound : N} : EqDecision (BoundedN bound).
+    Proof.
+      intros x y.
+      destruct (BoundedN.eqb_spec x y); [left|right]; assumption.
+    Qed.
+
+    Global Instance BoundedNEqDec {bound : N} : EqDecision (BoundedN bound) :=
+      eq_dec.
+
+    Definition encode_bounded {bound : N} (n : BoundedN bound) : positive :=
+      encode (to_N n).
+
+    Definition decode_bounded {bound : N} (n : positive) : option (BoundedN bound) :=
+      decode n >>= of_N.
+
+    Lemma decode_encode_bounded {bound : N} (n : BoundedN bound) :
+      decode_bounded (encode_bounded n) = Some n.
+    Proof.
+      unfold decode_bounded, encode_bounded.
+      rewrite decode_encode.
+      simpl.
+      apply of_to_N.
+    Qed.
+
+    Global Instance BoundedNCountable {bound : N} : Countable (BoundedN bound) :=
+      {| encode := encode_bounded;
+         decode := decode_bounded;
+         decode_encode := decode_encode_bounded; |}.
+  End Stdpp.
+
+  Global Instance BoundedN_finite {bound : N} : Finite (BoundedN bound) :=
+    {| elements := map_option of_nat (List.seq 0 (N.to_nat bound)) |}.
+  Proof.
+    - pose proof (seq_NoDup (N.to_nat bound) 0) as nodup.
+      pose proof (in_seq (N.to_nat bound) 0) as in_seq'.
+      pose proof (fun n => proj1 (in_seq' n)) as in_seq; clear in_seq'.
+      induction nodup; try constructor.
+      simpl.
+      pose proof (in_seq x) as x_bound.
+      specialize (x_bound (or_introl eq_refl)).
+      destruct x_bound as [useless x_bound]; clear useless.
+      simpl in x_bound.
+      destruct (of_nat x) eqn:ofnatx. all: cycle 1.
+        apply of_nat_none in ofnatx.
+        lia.
+      constructor.
+      + intros Hin.
+        apply in_map_of_nat in Hin.
+        apply of_nat_some in ofnatx.
+        rewrite <- ofnatx in H.
+        tauto.
+      + apply IHnodup.
+        intros n in_n_l.
+        apply (in_seq n (or_intror in_n_l)).
+    - intros t.
+      apply in_map_of_nat.
+      apply in_seq.
+      unfold to_nat.
+      destruct t as [t lt].
+      simpl.
+      change ((bound ?= t) = Gt) with (bound > t) in lt.
+      lia.
+  Qed.
+End BoundedN.
+
+Delimit Scope BoundedN_scope with BoundedN.
+Bind Scope BoundedN_scope with BoundedN.
