src/Circulation.v
@@ -1,0 +1,178 @@
+(* In this file we prove various results about the circulation of coins in any
+chain implementing a chain type. More specifically, we show that the circulation
+does not change during execution of blocks. This is proven under the (implicit)
+assumption that the address space is finite. *)
+From Coq Require Import List Permutation ZArith Psatz.
+From SmartContracts Require Import Automation Blockchain Extras Finite.
+From RecordUpdate Require Import RecordSet.
+Import ListNotations.
+
+Section Circulation.
+Context {ChainBaseTypes : ChainBaseTypes}.
+Context `{Finite Address}.
+
+Definition circulation (chain : Chain) :=
+  sumZ (account_balance chain) (elements Address).
+
+Definition coins_created (start_height end_height : nat) : Amount :=
+  sumZ compute_block_reward (seq (S start_height) (end_height - start_height)).
+
+(* We then prove that over any single step, the circulation is preserved.
+The idea behind this proof is that addrs contain from and to so
+we can move them to the beginning of the sum and it easily follows that
+the sum of their balances is the same as before. For the rest of the
+list the total balance will then not be affected which follows by induction. *)
+Lemma address_reorganize {a b : Address} :
+  a <> b ->
+  exists suf, Permutation ([a; b] ++ suf) (elements Address).
+Proof.
+  intros a_neq_b.
+  apply (NoDup_incl_reorganize _ [a; b]);
+    repeat constructor; unfold incl; prove.
+Qed.
+
+Lemma step_from_to_same
+      {pre : Environment}
+      {act : Action}
+      {tx : Tx}
+      {post : Environment}
+      {new_acts : list Action}
+      (step : ChainStep pre act tx post new_acts) :
+  tx_from tx = tx_to tx ->
+  circulation post = circulation pre.
+Proof.
+  intros from_eq_to.
+  unfold circulation.
+  induction (elements Address) as [| x xs IH].
+  - reflexivity.
+  - simpl in *.
+    rewrite IH, (account_balance_post step), from_eq_to.
+    lia.
+Qed.
+
+Hint Resolve step_from_to_same.
+
+Lemma step_circulation_unchanged
+      {pre : Environment}
+      {act : Action}
+      {tx : Tx}
+      {post : Environment}
+      {new_acts : list Action}
+      (step : ChainStep pre act tx post new_acts) :
+  circulation post = circulation pre.
+Proof.
+  destruct (address_eqb_spec (tx_from tx) (tx_to tx))
+    as [from_eq_to | from_neq_to]; eauto.
+  destruct (address_reorganize from_neq_to) as [suf perm].
+  apply Permutation_sym in perm.
+  unfold circulation.
+  rewrite 2!(sumZ_permutation perm); prove.
+  rewrite (account_balance_post_to step from_neq_to).
+  rewrite (account_balance_post_from step from_neq_to).
+  enough (sumZ (account_balance pre) suf = sumZ (account_balance post) suf) by prove.
+
+  pose proof (Permutation_NoDup perm) as perm_set.
+  assert (from_not_in_suf: ~In (tx_from tx) suf).
+  { apply (in_NoDup_app _ [tx_from tx; tx_to tx] _); prove. }
+  assert (to_not_in_suf: ~In (tx_to tx) suf).
+  { apply (in_NoDup_app _ [tx_from tx; tx_to tx] _); prove. }
+
+  clear perm perm_set.
+  pose proof (account_balance_post_irrelevant step).
+  induction suf as [| x xs IH]; prove.
+Qed.
+
+Hint Resolve step_circulation_unchanged.
+
+(* Finally, we get the result over block traces by a simple induction. *)
+Lemma block_trace_circulation_unchanged
+      {bef : list Action}
+      {after : list Action}
+      {post pre : Environment}
+      (trace : BlockTrace pre bef post after)
+  : circulation post = circulation pre.
+Proof.
+  induction trace;
+    match goal with
+    | [IH: _ |- _] => try rewrite IH; eauto
+    end.
+Qed.
+
+Hint Resolve block_trace_circulation_unchanged.
+
+Lemma circulation_equal (c1 c2 : Chain) :
+  ChainEquiv c1 c2 -> circulation c1 = circulation c2.
+Proof.
+  intros [].
+  unfold circulation, account_balance.
+  induction (elements Address); prove.
+Qed.
+
+Lemma circulation_add_new_block header baker env :
+  circulation (add_new_block header baker env) =
+  (circulation env + compute_block_reward (block_height header))%Z.
+Proof.
+  assert (Hperm: exists suf, Permutation ([baker] ++ suf) (elements Address)).
+  { apply NoDup_incl_reorganize; repeat constructor; unfold incl; prove. }
+  destruct Hperm as [suf perm].
+  symmetry in perm.
+  pose proof (Permutation_NoDup perm (elements_set Address)) as perm_set.
+  unfold circulation.
+  rewrite perm.
+  simpl.
+  unfold constructor, set, account_balance.
+  simpl.
+  destruct (address_eqb_spec baker baker); try congruence.
+  simpl.
+  pose proof (in_NoDup_app baker [baker] suf ltac:(prove) perm_set) as not_in_suf.
+  repeat rewrite <- Z.add_assoc.
+  f_equal.
+  rewrite <- Z.add_comm.
+  repeat rewrite <- Z.add_assoc.
+  f_equal.
+
+  clear perm perm_set e.
+  induction suf as [| x xs IH]; auto.
+  simpl in *.
+  apply Decidable.not_or in not_in_suf.
+  destruct (address_eqb_spec x baker); try tauto.
+  specialize (IH (proj2 not_in_suf)).
+  lia.
+Qed.
+
+Theorem chain_trace_circulation
+      {env_start env_end : Environment}
+      (trace : ChainTrace env_start env_end)
+  : circulation env_end =
+    (circulation env_start +
+     coins_created
+       (block_height (block_header env_start))
+       (block_height (block_header env_end)))%Z.
+Proof.
+  unfold coins_created.
+  induction trace as
+      [|prev_start prev_end header baker acts block_start new_end prev_trace IH valid block_trace eq].
+  - rewrite Nat.sub_diag.
+    simpl. lia.
+  - unfold IsValidNextBlock in valid.
+    rewrite (block_header_post_steps block_trace).
+    rewrite (chain_equiv _ _ eq).
+    simpl.
+    rewrite (proj1 valid).
+    unfold coins_created.
+    pose proof (block_height_post_trace prev_trace) as height_le.
+    match goal with
+    | [|- context[S ?a - ?b]] => replace (S a - b) with (S (a - b)) by lia
+    end.
+    rewrite sumZ_seq_S.
+    unfold coins_created in IH.
+    rewrite Z.add_assoc, <- IH.
+    match goal with
+    | [|- context[S ?a + (?b - ?a)]] => replace (S a + (b - a)) with (S b) by lia
+    end.
+    rewrite (block_trace_circulation_unchanged block_trace).
+    rewrite (circulation_equal _ _ eq).
+    rewrite circulation_add_new_block.
+    now rewrite (proj1 valid).
+Qed.
+End Circulation.
