src/Containers.v
@@ -1,8 +1,8 @@
-From Coq Require Import ProofIrrelevance.
+From Coq Require Import List.
 From Coq Require Import ZArith.
 From stdpp Require gmap.
-From Coq Require Import List.
 From SmartContracts Require Import Monads.
+From SmartContracts Require Import BoundedN.
 Import ListNotations.
 
 Notation FMap := gmap.gmap.
@@ -22,16 +22,54 @@ Module FMap.
   Notation elements := fin_maps.map_to_list.
   Notation size := stdpp.base.size.
   Notation of_list := fin_maps.list_to_map.
+  Notation union := stdpp.base.union.
+  Notation alter := stdpp.base.alter.
+  Notation partial_alter := stdpp.base.partial_alter.
 
-  Proposition of_elements_eq
-              {A B : Type}
-              `{countable.Countable A}
-              (m : FMap A B)
-              : of_list (elements m) = m.
-  Proof.
-    apply fin_maps.list_to_map_to_list.
-  Qed.
+  Section Theories.
+    Context {K V : Type} `{countable.Countable K}.
+
+    Proposition of_elements_eq (m : FMap K V) :
+      of_list (elements m) = m.
+    Proof. apply fin_maps.list_to_map_to_list. Qed.
+
+    Lemma find_union_None (m1 m2 : FMap K V) (k : K) :
+      find k m1 = None ->
+      find k m2 = None ->
+      find k (union m1 m2) = None.
+    Proof.
+      intros find1 find2.
+      apply fin_maps.lookup_union_None; auto.
+    Qed.
+
+    Lemma find_union_Some_l (m1 m2 : FMap K V) (k : K) (v : V) :
+      find k m1 = Some v ->
+      find k (union m1 m2) = Some v.
+    Proof. apply fin_maps.lookup_union_Some_l. Qed.
+
+    Lemma find_add (m : FMap K V) (k : K) (v : V) :
+      find k (add k v m) = Some v.
+    Proof. apply fin_maps.lookup_insert. Qed.
+
+    Lemma find_add_ne (m : FMap K V) (k k' : K) (v : V) :
+      k <> k' -> find k' (add k v m) = find k' m.
+    Proof. apply fin_maps.lookup_insert_ne. Qed.
+
+    Lemma find_partial_alter (m : FMap K V) f k :
+      find k (partial_alter f k m) = f (find k m).
+    Proof. apply fin_maps.lookup_partial_alter. Qed.
+
+    Lemma find_partial_alter_ne (m : FMap K V) f k k' :
+      k <> k' ->
+      find k' (partial_alter f k m) = find k' m.
+    Proof. apply fin_maps.lookup_partial_alter_ne. Qed.
+  End Theories.
 End FMap.
+
+Hint Resolve FMap.find_union_None.
+Hint Resolve FMap.find_union_Some_l.
+Hint Resolve FMap.find_add.
+Hint Resolve FMap.find_add_ne.
 
 Instance empty_set_eq_dec : stdpp.base.EqDecision Empty_set.
 Proof. decidable.solve_decision. Defined.
