src/Finite.v
@@ -1,0 +1,15 @@
+From Coq Require Import List.
+Import ListNotations.
+
+Class Finite (T : Type) :=
+  build_finite {
+    elements : list T;
+    elements_set : NoDup elements;
+    elements_all : forall (t : T), In t elements;
+  }.
+
+Arguments elements _ {_}.
+Arguments elements_set _ {_}.
+Arguments elements_all _ {_}.
+
+Hint Resolve elements_set elements_all.
